Makefile
@@ -8,11 +8,11 @@ EXTRACTED_FILES = \
 
 PROOF_FILES += $(EXTRACTED_FILES)
 PROOF_FILES += $(wildcard proof/*.ec)
+PROOF_FILES += $(wildcard proof/schnorr_protocol/*.ec)
 PROOF_FILES += $(wildcard proof/modular_multiplication/*.ec)
 PROOF_FILES += $(wildcard proof/montgomery_ladder/*.ec)
 PROOF_FILES += $(wildcard proof/rejection_sampling/*.ec)
 PROOF_FILES += $(wildcard proof/finite_types/*.ec)
-#PROOF_FILES += $(wildcard proof/schnorr_protocol/*.ec)
 PROOF_FILES += $(wildcard proof/definition_analysis/*.ec)
 
 
